Learn.LowStar.Util.fst
@@ -1,0 +1,24 @@
+module Learn.LowStar.Util
+
+module M   = LowStar.Modifies
+module HS  = FStar.HyperStack
+module U32 = FStar.UInt32
+
+(* necessary for hint replay *)
+noextract inline_for_extraction
+let u32_zero : x: U32.t {U32.v x == 0}
+  = U32.uint_to_t 0
+
+(* force a proof of [M.modifies] by transitivity *)
+#push-options "--ifuel 1"
+noextract noeq type mod_seq (#mod : M.loc) : HS.mem -> HS.mem -> Type =
+  | MNil  : h : HS.mem -> mod_seq #mod h h
+  | MCons : h0 : HS.mem -> #h1 : HS.mem -> #h2 : HS.mem ->
+               #squash (M.modifies mod h0 h1) -> mod_seq #mod h1 h2 -> mod_seq #mod h0 h2
+
+let rec mod_of_seq (mod : M.loc) (#h0 #h1 : HS.mem) (sq : mod_seq #mod h0 h1)
+  : Lemma (ensures M.modifies mod h0 h1) (decreases sq)
+  = match sq with
+    | MNil _ -> ()
+    | MCons _ sq -> mod_of_seq mod sq
+#pop-options
